Iris/Iris/Tests.lean
@@ -6,4 +6,5 @@ public import Iris.Tests.Notation
 public import Iris.Tests.Tactics
 public import Iris.Tests.HeapLang
 public import Iris.Tests.Language
+public import Iris.Tests.TotalWeakestPre
 public import Iris.Tests.WeakestPre
